% \subsection{Stability and Equilibrium Points}

% \subsubsection{Equilibrium Points}

% Given the system:

% $$
% \begin{cases}
%     \dot x = f(x) \\
%     x \in \mathbb{R}^n
% \end{cases}
% $$

% An equilibrium point is a point $x^*$ such that $f(x^*) = 0$.

% \begin{tipsblock}[Eq. points]
% A system can have multiple equilibrium points.
% \end{tipsblock}

% We have three kinds of equilibrium:

% \begin{itemize}
%     \item \textbf{Stable equilibrium}: if the system is in the neighborhood of the equilibrium point, it will remain there.
%     \item \textbf{Neutral equilibrium}: if the system is in the neighborhood of the equilibrium point, it will remain there, but it will not return to it.
%     \item \textbf{Unstable equilibrium}: if the system is in the neighborhood of the equilibrium point, it will move away from it.
% \end{itemize}

% \begin{figure}[H]
%     \centering
%     \includegraphics[width=0.65\textwidth]{assets/eq_points.png}
%     \caption{Stable, Natural and Unstable Equilibrium Points \cite{stability}}
% \end{figure}

% \subsubsection{Stability}

% We say that a system is \textbf{\textit{Globally Asymptotically Stable}} (or \textit{Globally Attractive}) if it is stable and if it converges to the equilibrium point from any initial condition.

% \subsection{Local Analysis Near the Equilibrium Point}

% In this section, we study the system in the neighborhood of the equilibrium point. Let the initial condition be a small perturbation around the equilibrium:

% $$
% X(0) = X_e + \varepsilon.
% $$

% We introduce a deviation function $U(t)$ defined by

% $$
% X(t) = X_e + U(t),
% $$

% with the initial condition

% $$
% U(0) = \varepsilon.
% $$

% Thus, the evolution of the perturbation is governed by

% $$
% \begin{cases}
% \dot U = f(X_e + U), \\
% U(0) = \varepsilon.
% \end{cases}
% $$

% Assume that the dynamics of the system are given by

% $$
% \dot X = X(b(X) - m(X)).
% $$

% Then the perturbed system becomes

% $$
% \dot U = (b(X_e + U) - m(X_e + U))(X_e + U).
% $$

% Expanding $b(X_e + U)$ and $m(X_e + U)$ in a Taylor series around $X_e$, we have:

% $$
% b(X_e + U) \approx b(X_e) + b'(X_e)U,
% $$
% $$
% m(X_e + U) \approx m(X_e) + m'(X_e)U.
% $$

% Substituting these into the equation for $\dot U$, we get:

% $$
% \begin{array}{rl}
% \dot U & = \bigl[b(X_e) + b'(X_e)U\bigr] - \bigl[m(X_e) + m'(X_e)U\bigr](X_e + U) \\
%       & = \bigl[b(X_e) + b'(X_e)U\bigr] - \bigl[m(X_e)X_e + m(X_e)U + m'(X_e)X_eU + m'(X_e)U^2\bigr].
% \end{array}
% $$

% Since the equilibrium condition implies that

% $$
% (b(X_e) - m(X_e))X_e = 0,
% $$

% the above expression simplifies (neglecting the higher-order term $m'(X_e)U^2$) to:

% $$
% \dot U \approx \left[b'(X_e) - m(X_e) - m'(X_e)X_e\right] U.
% $$

% Under the assumption that $b'(X_e)$ is negative, we can express this as

% $$
% \dot U \approx -X_e\Bigl(|b'(X_e)| + m'(X_e)\Bigr)U.
% $$

% The solution of this linearized differential equation is given by:

% $$
% U(t) = U(0)\,e^{-X_e (|b'(X_e)| + m'(X_e))t}.
% $$

% Hence, we identify the decay rate (or the inverse of the characteristic time constant) as

% $$
% X_e\Bigl(|b'(X_e)| + m'(X_e)\Bigr),
% $$

% and the characteristic time $\tau$ is:

% $$
% \tau = \frac{1}{X_e \left(|b'(X_e)| + m'(X_e)\right)}.
% $$

% This time constant represents the rate at which perturbations decay in the vicinity of the equilibrium point.


% \newpage

% $$
% X(t) = X_e + U(t) \Rightarrow \dot U = f(X_e + U) = \underbrace{f(X_e)}_{=\ 0} + f'(X_e)U + O(U^2)
% $$

% $$
% \dot U = f'(X_e)U \Rightarrow U(t) = U(0) e^{f'(X_e)t}
% $$

% So we have:
% $$
% \begin{cases}
% f'(X_e) < 0 \quad \Rightarrow \quad X_e \text{ is Locally Asintotically stable } \\
% f'(X_e) > 0 \quad \Rightarrow \quad X_e \text{ is Unstable }
% \end{cases}
% $$

% \vspace{2em}

% \section{Non-scalar Systems}

% Consider the system:

% $$
% \begin{cases}
%     \dot x = f(x) \\
%     x \in \mathcal{f} \subseteq \mathbb{R}^n
% \end{cases}
% $$

% As in the scalar case, we can linearize the system around the equilibrium point $x_e$:

% $$
% f(X_e) = 0
% $$

% $$
% X = X_e + U, \quad \quad |U| \ll 1
% $$

% We have to consider the Jacobian matrix of $f$:

% \dots

% \subsection{Exponential of a Matrix}

% Let's consider a linear system of the form:

% $$
% \dot x = Ax
% $$

% where $A \in \mathbb{R}^{n \times n}$ is a matrix. The solution of this system is given by:

% $$
% x(t) = e^{At} x(0)
% $$

% where $e^{At}$ is the exponential of the matrix $A$.

% \begin{definitionblock}[Exponential of a Matrix]
% Given a matrix $A \in \mathbb{R}^{n \times n}$, the exponential of $A$ is defined as:

% $$
% e^A = I + A + \frac{A^2}{2!} + \frac{A^3}{3!} + \dots = \sum_{k=0}^{\infty} \frac{A^k}{k!}
% $$

% This comes from the Taylor series expansion of the exponential function.
% \end{definitionblock}

% $$
% \dfrac d{dt} e^{At} = \sum_{m = 1}^\infty A^m m \dfrac{t^{m-1}}{m(m-1)!}
% = \sum_{k = 0}^\infty A A^k \dfrac{t^k}{k!}
% = A e^{At}
% $$

% $$
% \begin{array}{lll}
% A & = & H \cdot \text{Diag}(\lambda_1, \lambda_2, \dots, \lambda_n) \cdot H^{-1} \\
% A^2 & = & H \cdot \text{Diag}(\lambda_1^2, \lambda_2^2, \dots, \lambda_n^2) \cdot H^{-1} \\
% A^m & = & H \cdot \text{Diag}(\lambda_1^m, \lambda_2^m, \dots, \lambda_n^m) \cdot H^{-1}
% \end{array}
% $$

% So we have:

% $$
% e^{At} = \sum_{m = 0} ^ \infty \dfrac{A^m t^m}{m!} = 
% $$

