


\newpage

\section{Liouville Equation for Systems with Uncertain Initial Conditions}

Consider a physical system governed by the ordinary differential equation
$$
\begin{cases}
\displaystyle \frac{dx}{dt} = a(x),\\[1mm]
x(0)=x_0,
\end{cases}
$$
where the initial condition $x_0$ is not known exactly. Instead, we assume that $x_0$ is drawn from a probability distribution $\theta(x_0)$, so that the system is defined by
$$
\begin{cases}
\displaystyle \frac{dx}{dt} = a(x),\\[1mm]
x(0)=x_0 \sim \theta(x_0).
\end{cases}
$$

Suppose there exists an equilibrium point $x_e$ such that $a(x_e)=0$, and that $x_e$ is globally asymptotically stable (G.A.S.). This implies that, regardless of the uncertainty in the initial condition, the state $x(t)$ converges to $x_e$ as $t\to\infty$. Consequently, the probability density function (PDF) $\rho(x,t)$ of $x(t)$ evolves towards a Dirac delta distribution centered at $x_e$:
$$
\lim_{t\to\infty} \rho(x,t) = \delta(x-x_e).
$$

The time evolution of $\rho(x,t)$ is governed by the \textbf{Liouville equation}. For the deterministic dynamics
$$
dx = a(x)\,dt,
$$
the Liouville equation is given by
$$
\frac{\partial \rho}{\partial t} = - \frac{\partial}{\partial x}\Bigl[a(x)\,\rho(x,t)\Bigr].
$$

This partial differential equation expresses the conservation of probability along the flow of the system. The term $-\frac{\partial}{\partial x}\left[a(x)\,\rho(x,t)\right]$ represents the net flux of probability density in the state space due to the vector field $a(x)$. As time evolves and the system converges to the stable equilibrium $x_e$, the density $\rho(x,t)$ becomes increasingly concentrated around $x_e$, reflecting the loss of uncertainty in the long-term behavior of the system.

\newpage

\begin{align}
    m\dot v &= - \gamma v + F_s(t) \tag{I}\\
    Ri &= -L \dfrac{di}{dt} - K \dfrac{dB_{ext}}{dt} \tag{II}\\
    m \ddot x &= - \hat k x - \gamma \dot x + \hat F(t) \tag{III}
\end{align}

\dots

$$
\dot z = - \gamma z + \omega \xi(t) \leftrightarrow dz = . \gamma z dt + \omega \xi(t) dt \quad \Rightarrow \quad z = e^{- \gamma t} Q
$$

$$
- \gamma e^{\gamma t} Q dt + e^{-\gamma t} dQ = - \gamma e ^ {- \gamma t} Q + \omega dW
\quad \Rightarrow \quad 
e^{-\gamma t}dz = \omega dW
$$

So we have:

$$
dQ = e^{\gamma t} \omega dW \quad = \quad Q(t) = z(0) + \omega \int_{0}^{t} e^{\gamma s} dW(s) 
\quad \Rightarrow \quad
\boxed{
z(t) = z_0 e^{- \gamma t} + \omega \int_0^t e^{\gamma (s-t)} dW(s)
}
$$

$$
\langle z(t) \rangle = \langle z_0 \rangle e^{-\gamma t} + \Phi
$$

\dots

$$
z(t) = z(0)e^{- \gamma t} + \omega \int_0^t e^{\gamma (s-t)} dW(s)
$$

$$
\begin{array}{rl}
\langle z^2(t) \rangle =& 
\left\langle 
    \left(
        z_0 e^{-\gamma t} dW(s) + \int_0^t e^{\gamma(s - t)} \xi(s)ds
    \right)
    \left(
        z_0 e^{-\gamma t} + \int_0^t e^{\gamma(\theta - t) \xi(\theta)d\theta}
    \right)
\right\rangle
\\
=&
\left\langle
    \left(
        z_0 ^2 e^{-2\gamma t} + z_0 e^{-\gamma t} \int_0^t e^{\gamma(\theta - t)} \xi(\theta)d\theta + z_0 e^{-\gamma t} \int_0^t e^{\gamma(s - t)} \xi(s)ds + J(t)
    \right)
\right\rangle
\\
=&
\dots
\end{array}
$$

$$
\begin{array}{rl}
    \langle J(t) \rangle =& \omega^2 \int_0^t \int_0^t e^{\gamma(\theta + s - 2t)} \delta(\theta - s) d\theta ds\\
    =&
    \omega^2 e^{-2\gamma t} \int_0^t
     \left\{
        \int_0^t e^{\gamma(\theta + s)} \delta(\theta - s) d\theta 
    \right\}
    ds\\
    =&
    \omega^2 e^{-2\gamma t} \int_0^t e^{2 \gamma s} ds \\
    =&
    \omega^2 e^{-2\gamma t} \left[\dfrac{e^{2 \gamma t} - 1}{2 \gamma}\right] \\
    =&
    \dfrac{\omega^2}{2 \gamma} \big(1 - e^{-2 \gamma t}\big)
\end{array}
$$

$$
Var[z(t)] = \underbrace{\langle z_0^2 \rangle e^{-2 \gamma t} - (\langle z_0 \rangle)^2 e^{-2 \gamma t}}_{= \ Var(z_0)e^{-2 \gamma t}} + \dfrac{\omega^2}{2 \gamma} \big(1 - e^{-2 \gamma t}\big) = Var(z_0) e^{-2 \gamma t} + \dfrac{\omega^2}{2 \gamma} \big(1 - e^{-2 \gamma t}\big)
$$

$$
Var(z(t)) \to \dfrac {\omega}{2 \gamma} = \sigma^2
$$

$$
z(t) = e^{-\gamma t} + \int _0^t e^{\gamma(s-t)} \xi(s)dt
$$

\dots

$$z(0) = 0$$

$$
\langle z(t) z(q) \rangle = \omega^2 e^{-\gamma (t + q)} \int_0^t \int_0^q e^{\gamma(\theta + s)} \delta(\theta - s) d\theta ds
$$

We have 2 cases:

\begin{itemize}
    \item $\boldsymbol{t < q}$: 
    
        $$
        \langle z(t) z(q) \rangle = \omega^2 e^{-\gamma (t + q)} \int_0^t e^{2 \gamma s} ds 
        =
        \dfrac{\omega^2}{2 \gamma} e^{-\gamma (t - q)} \dots
        $$
        $$
        \langle z(t) z(q) \rangle = \dfrac{\omega^2}{2 \gamma} \left( e^{-\gamma |q - t|} - e^{-\gamma (q + t)} \right)
        $$

---

        $$
        z_0 = 0
        \quad
        \begin{cases}
        \langle z(t) \rangle = 0
        \\
        \langle z(q) \rangle = 0
        \end{cases}
        \quad
        C[\alpha, \beta] = \langle (\alpha - \hat \alpha)(\beta - \hat \beta) \rangle
        $$

        $$
        \rightarrow C[z(t), z(q)]; \quad q = t + h \quad X[z(t), z(t+h)] = \dfrac{\omega^2}{2 \gamma} \left( e^{-\gamma |h|} - e^{-\gamma h} e^{-2 \gamma t} \right)
        $$
        
        $$
        R_z(h) = \lim_{t \to \infty} C[z(t), z(t+h)] = \dfrac{\omega^2}{2 \gamma} e^{-\gamma |h|}
        $$
        
    \item $t > q$:
    

\end{itemize}