\chapter{Lecture 28/03/2025}

\dots

$$
\dfrac {di} {dt} = - \dfrac RL i + \omega \xi_1(t) + \dfrac KL i \xi_2 (t)
$$



Suppose to have an equation $dx = a(x) dt + b_1(X)dW_1 + b_2(x)dW_2$

Then 

$$
\dfrac {\partial}{\partial t} P(x, t) = - \dfrac{\partial}{\partial x} [a(x)P] + \dfrac{\partial^2}{\partial x^2} 
\left[
    \dfrac{b_1^2(x) b_2^2(x)}{2} P(x,t)
\right]
$$



$$
\begin{cases}
    \dfrac {dx}{dt} = f(x)\\
    x(0) \sim \theta(X_0)
\end{cases}
\quad \rightarrow \quad
\begin{cases}
    dx = f(x)dt + OdW\\
    \rho(x,0) = \theta(x)
\end{cases}
$$

$$
\begin{cases}
    \dfrac{\partial \rho}{\partial t} = - \dfrac{\partial}{\partial x} [f(x) \rho] \\
    \rho(x,0) = \theta(x)\\
    \int_{\Omega} \rho(x,t) dx = 1 
\end{cases}
$$

\begin{exampleblock}{Spring}
    Let's consider the following SDE describing the motion of a particle moved by a spring force.
    $$
    \begin{cases}
        \dfrac {dx}{dt} = -kx\\
        x(0) \sim \mathcal N (\mu = 1.8, \sigma^2 = 0.05)
    \end{cases}
    $$

    The solution of the SDE is given by:
    $$
    x(t) = x_0 e^{-kt} \quad \Rightarrow \quad x(t) \to 0
    $$
\end{exampleblock}

\rule{\textwidth}{0.4pt}

\newpage

\begin{exampleblock}[Stochastic Miultistability]

    Let's consider the following SDE describing the motion of a particle in a double well potential.
    
    $$
    \dot x = x - x^3 = x(1-x^2)
    $$
    
This system has three equilibrium points:

$$
\begin{cases}
    x_L = -1  & \quad \Rightarrow LAS\\
    x_C = 0  & \quad \Rightarrow Unstable\\
    x_R = + 1 & \quad \Rightarrow LAS
\end{cases}
$$

Where $LAS$ means locally asymptotically stable.

$$
\begin{cases}
    F = - \dfrac {dU}{dx} \\
    U(x) = \dfrac {-x^2}{2} + \dfrac {x^4}{2}
\end{cases}
$$


We can calculate the limit of the probability density function $\rho(x,t)$ as $t \to \infty$.

$$
\lim_{t \to \infty} \rho (x,t) = A_N \delta(x + 1) + A_P \delta(x - 1) + C \delta(x)
$$

Where $A_N$ and $A_P$ are the normal and particular solutions of the system:

$$
\begin{cases}
    A_P = \int_0^\infty \theta(x) dx = \Pr[x_0 > 0]\\
    A_N = \int_{-\infty}^0 \theta(x) dx =  \Pr[x_0 < 0]\\
    C = \Pr[x_0 = 0] = 0
\end{cases}
$$
\end{exampleblock}



\dots

$$\dot x = x - x^3 + \omega \xi(t)$$

$$
\dot x = - \dfrac {dU}{dx} + \omega \xi(t)
$$

$$
P_s(x) = A e^{-\dfrac 2 {\omega^2} U(x)}
$$

Role of $\omega$:

\begin{enumerate}
    \item $\omega \ll 1$: we have small obscillations so we can use the linear approximation of the system. The system is stable and we have a single peak in the probability density function.
    \item $\omega \gg 1$: we have large obscillations and in this case we can use the linear approximation of the system. The system is unstable and we have two peaks in the probability density function.
    $$
    P_s(x) = A_s e^{-\frac 2 {\omega^2}} \approx 1 
    $$
\end{enumerate}

\begin{observationblock}
    Matematically it is possible to say that after a very long period of time, also the first case we could see that the system moves from one peak to the other. This is due to the fact that the system is not stable and we have a non-zero probability of moving from one peak to the other. 
\end{observationblock}

$$
\dfrac{di}{dt} = - \dfrac {R i + k \xi_1(t)}L + \omega  \xi_2(t) = - \dfrac RL - \dfrac KL i \xi_2(t) + \omega \xi_1(t)
$$

\subsubsection{multiplicative noise}

The general form of a SDE with multiplicative noise is given by:

$$
dx = fx dt + g(x) dW
$$

We already saw a case of multiplicative noise:

$$
\dot x = (r_1 + \omega \xi(t))x - r_2 x^2 \quad \rightarrow \quad dx = \underbrace{(r_1 x - r_2 x^2)}_{f(x)}dt + \underbrace{\omega x}_{g(x)} dW
$$

$$
\dfrac{\partial \rho}{\partial t} = - \dfrac{\partial}{\partial x} [f(x) \rho] + \dfrac{\partial ^2}{\partial x^2} \left[ \dfrac{g^2(x)}{2} \rho \right]
$$

$$
\dfrac{d^2}{dx^2} \left[ \dfrac{g^2(x)}{2} \rho \right] = - \dfrac d{dx} [f(x)P_s]
$$

$$
\begin{cases}
    \dfrac{d}{dx} \left[ \dfrac{g^2(x)}{2} \rho \right] = - f(x)P \\
    Q(x) = \dfrac{g^2(x)}{2} \rho \quad \Rightarrow \quad P = \dfrac 2 {g^2(x)} Q
\end{cases}
$$
$$
\dfrac{dQ}{dx} = - f(x) \dfrac 2 {g^2(x)} Q
$$
$$
\dfrac{dy}{dx} = a(x) y \quad \Rightarrow \quad
\begin{cases}
    y(x) = Ce^{A(x)}\\
    A(x) = \int_\alpha^x a(s) ds
\end{cases}
$$
$$
Q(x) = C \exp\left\{
    \int_\alpha^x - \dfrac{2 f(s)}{g^2(s)} ds
\right\}
\quad \Rightarrow \quad
P(x) = \dfrac{2}{g^2(x)} \exp \left\{
    \int_\alpha^x \dfrac{2 f(z)}{g^2(z)} dz
\right\}
$$

Now we have to derivate the probability density function, before doing this, let's rewrite it in a way that simplifies calculus.

Considering that:

$$
\dfrac 1{g^2(x)} = e^{-\ln g^2(x)} = e^{-2 \ln g(x)}
$$

We can rewrite the probability density function as:

$$
P(x) = 2 C \exp \left\{
    - 2 \log (g(x)) + \int_\alpha^x \dfrac{2 f(s)}{g^2(s)} ds
\right\}
$$

Now we can derivate:

$$
P'(x) = 2 C \exp \left\{
    - 2 \dfrac{g'(x)}{g(x)} + \dfrac{2 f(x)}{g^2(x)}
    \right\}
$$

\dots

$$
\boxed{f(x) \ge g'(x)g(x)}
$$

\dots

$$
g(x) = \omega \Rightarrow P'_s(x) \ge 0 \equiv f(x) \ge 0 \qquad - \dfrac {dU}{dx} \ge 0
$$

As results we have that:

\begin{enumerate}
    \item Extrema of $P_s$ are different from extrema of $U(x)$ (= equoilibrium point of the deterministic system).
    
    \item The number of extrema of $P_s$ is different from the numnber of equilibrium points.
\end{enumerate}

\subsubsection{Something biological idk why}

Proteins in our cells follows a self-assembly model. The model is given by the following SDE:

$$
\dfrac {dx}{dt} = \Pi_R(x) - \delta x
$$

where $\Pi_R(x)$ is the production rate of the protein.

The production rate is given by the following equation:

$$
\Pi_R(x) = R + \dfrac {k x^2}{k_0 + x^2}
$$

The equilibrium points are given by:

$$
\Pi_R(x) = \delta x
$$

Let's now consider $\delta = \delta + \alpha \xi(t)$, where $\alpha$ is a constant and $\xi(t)$ is a white noise.
We can rewrite the equation as:

$$
\dfrac{dx}{dt} = \left(
    R + k \dfrac{x^2}{k_0 + x^2} - \delta x
\right)
+ \alpha x \xi(t)
$$

In this case we have a multiplicative noise, so we can use the previous results, but now we do not have to intercept $\Pi_R$ with $\delta$, but we have to intercept it with $\delta + \alpha^2$.

$$
\begin{cases}
    R + k \dfrac{x^2}{k_0 + x^2} - \delta x \ge \alpha^2 x \\
    R + k \dfrac{x^2}{k_0 + x^2} \ge (\delta + \alpha^2) x
\end{cases}
$$

\newpage

$$\dot z = r_1 z - r_2 z, \qquad x = r_2 z \to z = \dfrac {x}{r_2}$$

$$
\begin{cases}
    \dot x = r_1 x - x^2 \\
    r_1 \to r_1 + \omega \xi(t)
\end{cases}
\quad \Rightarrow \quad
dx = (r_1 x - x^2) dt + \omega x dW
$$

$$
f(x) = r_1 x - x^2,
\qquad
g(x) = \omega x
$$

$$
r x - x^2 \ge \omega^2 x
\qquad \Rightarrow \qquad
r_1 - x \ge \omega^2
$$

in $\omega^2 = r_1$ we have a transition from an unimodal stationary distribution to a decreasing function.

$$
P_s = \dfrac {2C}{\omega^2} x^{2r_1/\omega^2 - 2}\ e^{-(2/\omega^2) x}
$$

which is not integrable

\subsubsection{voglio anna a casa}

$$
dx = f(x) dt + g(x) dW 
$$

$$
x(t + dt) = x(t) + f(x(t))dt + g(x(t)) G_t \sqrt{dt}
$$

We have that the probability of moving from $s$ to $a$ in a time $dt$ is given by:

$$
\Pr\left(x(t + dt) "=" a | x(t) = s\right) = \Omega(s, a) dt 
$$

While the probability of not moving is given by:

$$
\Pr\left(x(t + dt) "=" s | x(t) = s\right) = 1 - \int \Omega(s,a)dt 
$$


